---
Course: CALENG3
Status: Work in Progress
References used:
  - 1.1 Variable Separable (Lecture Slides)
  - 1.5 Homogeneous de (Lecture Slides)
tags:
  - lesson
---

- Variable Separable
	- General Form
		- $M(x,y)dx+N(x,y)dy=0$
		- The two functions must be products or quotients of x and y, meaning that they can be separated. Otherwise, they are not variable separable.
	- Solution
		- $A(x)B(y)dx+C(x)D(y)dy=0$
		- General Solution
			- $F(x,y)=c$
	- Solving steps
		1. Make sure that the functions $M$ and $N$ are products or quotients of $x$ and $y$, else they are not variable separable.
		2. Separate the variables by making $dx$ together with all the $x$s, and by making all the $y$s in the function together with $dy$. In other words, isolate the $x$ and $y$ from each other.
		3. Integrate
		4. The general solution would be in the form of $F(x,y)=c$, where $F$ is a function of $x$ and $y$, and $c$ is the constant of integration.
- DEs with Homogeneous Coefficient
	- Homogeneous Function
		1. A function is said to be homogeneous of degree $n$ if and only if
			- $f(tx,ty)=t^nf(x,y)$
			- You can draw out the original function multiplied by  $t^n$ when substituting $tx$ to $x$ and $ty$ to $y$ in the function.
		2. The DE $M(x,y)dx+N(x,y)dy=0$ is only homogeneous when both $M(x,y)$ and $N(x,y)$ are homogeneous, and are of the same degree.
			- Standard form
				- $M(x,y)dx+N(x,y)dy=0$
			- Solution
				- If $M$ is simpler than $N$
					1. let: $x=vy$
					2. let: $dx=vdy+ydv$
				- If $N$ is simpler than $M$
					1. let: $y=vx$
					2. let: $dy=vdx+xdv$
			- General Solution
				- $F(x,y)=c$
					- Substitution would reduce the resulting DE into a variable separable type.
	- Solving steps [(recommended video)](https://youtu.be/2DlgbW-mO0o?feature=shared)
		1. Check if the equation is homogeneous.
		2. For this example, $M$ is simpler than $N$, so let $x=vy$ and $dx=vdy+ydv$.
		3. Substitute the new values of $x$ and $dx$ to the homogeneous DE.
		4. Simplify the equation.
		5. Separate the variables (or isolate them from each other).
		6. Integrate
		7. Replace $v$ using $x=vy$, so $v=\frac{x}{y}$. This would slightly be different if $N$ was simpler than $M$ since it would use $y=vx$.
		8. The general solution would be in the form of $F(x,y)=c$, where $F$ is a function of $x$ and $y$, and $c$ is the constant of integration.
- Exact DEs
	- Given: $F(x,y)=0$
		- Total differential
			- $\frac{\partial F}{\partial x}dx+\frac{\partial F}{\partial y}dy=0$
		- General form of ODE
			- $M(x,y)dx+N(x,y)dy=0$
		- Therefore
			- $M(x,y)$
				1. $M(x,y)=\frac{\partial F}{\partial x}$
				2. $\frac{\partial M(x,y)}{\partial y}=\frac{\partial ^2F}{\partial y \partial x}$
			- $N(x,y)$
				1. $N(x,y)=\frac{\partial F}{\partial y}$
				2. $\frac{\partial N(x,y)}{\partial x}= \frac{\partial^2 F}{\partial x \partial y}$
	- For: $\frac{\partial ^2F}{\partial y \partial x} = \frac{\partial^2 F}{\partial x \partial y}$
		- Sufficient and necessary condition for exact DE
			- $\frac{\partial M(x,y)}{\partial y}=\frac{\partial N(x,y)}{\partial x}$
		- General solution
			- $F(x,y)=c$
	- Solving steps [(recommended video)](https://youtu.be/rNpMtelVVUQ?feature=shared)
		1. Test of exactness
			- In this step, get the partial derivative of the functions with respect to their opposite variables. So the partial derivative of $M(x,y)dx$ is $\frac{\partial M}{\partial y}$ and the partial derivative of $N(x,y)dy$ is $\frac{\partial N}{\partial x}$. Check if $\frac{\partial M}{\partial y}=\frac{\partial N}{\partial x}$, and if they are, it means that they are an exact DE.
		2. You can either solve using $M$ or $N$. For this example, we’ll use $M$. Replace the entire $N$ function and $dy$ to $g(y)$.
		3. Integrate the first function $M$ with respect to x because of the $dx$ in the function.
		4. Find the derivative of the entire equation with respect to y.
			- The derivative of $g(y)$ is $g'(y)$.
		5. Make the entire equation equal to the original value of second function (before changing it to $g(y)$), and solve for $g’(y)$.
		6. Integrate $g’(y)$ to get $g(y)$.
		7. Substitute the solved $g(y)$ to the whole equation found after doing step 3.
		8. The general solution would be in the form of $F(x,y)=c$, where $F$ is a function of $x$ and $y$, and $c$ is the constant of integration.